partial progress added to proof, unnecessary files deleted

arimthetic/src/main.rs
@@ -7,11 +7,11 @@ fn polynomial_factors1(x: i32) -> i32{
 }
 
 
-fn polynomial_factors2(x: u8) -> u8{
-    x*(x-2)
+fn polynomial_factors2(x: i32) -> i32{
+    x*(x-1)
 }
 
 
-fn polynomial(x: u8) -> u8{
+fn polynomial(x: i32) -> i32{
     x*x-x
 }
