arimthetic/target/hax/debug/deps/arimthetic-85d93f14f8655d40.d
@@ -1,6 +1,6 @@
-/Users/dc45624/Documents/GitHub/Formally-verifying-leetcode-solutions/arimthetic/target/hax/debug/deps/arimthetic-85d93f14f8655d40.d: src/main.rs
+/Users/dc45624/Documents/GitHub/Formally-verifying-leetcode-solutions/arimthetic_another_try/target/hax/debug/deps/arimthetic-85d93f14f8655d40.d: src/main.rs
 
-/Users/dc45624/Documents/GitHub/Formally-verifying-leetcode-solutions/arimthetic/target/hax/debug/deps/libarimthetic-85d93f14f8655d40.rmeta: src/main.rs
+/Users/dc45624/Documents/GitHub/Formally-verifying-leetcode-solutions/arimthetic_another_try/target/hax/debug/deps/libarimthetic-85d93f14f8655d40.rmeta: src/main.rs
 
 src/main.rs:
 
